Weidenbach_Book/IsaSAT_Lookup_Conflict.thy
@@ -734,21 +734,16 @@ sepref_thm set_lookup_conflict_aa_fast_code
     is_NOTIN_def[symmetric]
   apply (rewrite at \<open>_ + \<hole>\<close> annotate_assn[where A = \<open>uint32_nat_assn\<close>])
   supply [[goals_limit = 1]]
-  apply sepref_dbg_keep
-      apply sepref_dbg_trans_keep
-           apply sepref_dbg_trans_step_keep
-           apply sepref_dbg_side_unfold apply (auto simp: )[]
-
   by sepref
 
-concrete_definition (in -) set_lookup_conflict_aa_code
-   uses isasat_input_bounded.set_lookup_conflict_aa_code.refine_raw
+concrete_definition (in -) set_lookup_conflict_aa_fast_code
+   uses isasat_input_bounded.set_lookup_conflict_aa_fast_code.refine_raw
    is \<open>(uncurry6 ?f, _) \<in> _\<close>
 
-prepare_code_thms (in -) set_lookup_conflict_aa_code_def
+prepare_code_thms (in -) set_lookup_conflict_aa_fast_code_def
 
-lemmas set_lookup_conflict_aa_code[sepref_fr_rules] =
-   set_lookup_conflict_aa_code.refine[OF isasat_input_bounded_axioms]
+lemmas set_lookup_conflict_aa_fast_code[sepref_fr_rules] =
+   set_lookup_conflict_aa_fast_code.refine[OF isasat_input_bounded_axioms]
 
 lemma lookup_conflict_merge'_spec:
   assumes
@@ -1114,15 +1109,25 @@ proof -
     by (intro nres_relI frefI) (auto simp: H)
 qed
 
-theorem resolve_lookup_conflict_merge_code_set_conflict[sepref_fr_rules]:
-  \<open>(uncurry6 set_lookup_conflict_aa_code, uncurry6 set_conflict_m) \<in>
+theorem
+  resolve_lookup_conflict_merge_code_set_conflict[sepref_fr_rules]:
+    \<open>(uncurry6 set_lookup_conflict_aa_code, uncurry6 set_conflict_m) \<in>
   [\<lambda>((((((M, N), i), xs), clvls), lbd), outl). clvls = 0 \<and> i \<in># dom_m N \<and> xs = None \<and> distinct (N \<propto> i) \<and>
     literals_are_in_\<L>\<^sub>i\<^sub>n (mset (N \<propto> i)) \<and> \<not> tautology (mset (N \<propto> i)) \<and> literals_are_in_\<L>\<^sub>i\<^sub>n_trail M \<and>
      no_dup M \<and> out_learned M None outl]\<^sub>a
   trail_assn\<^sup>k *\<^sub>a clauses_ll_assn\<^sup>k *\<^sub>a nat_assn\<^sup>k *\<^sub>a option_lookup_clause_assn\<^sup>d *\<^sub>a uint32_nat_assn\<^sup>k *\<^sub>a
       lbd_assn\<^sup>d *\<^sub>a out_learned_assn\<^sup>d \<rightarrow>
     option_lookup_clause_assn *a uint32_nat_assn *a lbd_assn *a out_learned_assn\<close>
-   (is \<open>?c \<in> [?pre]\<^sub>a ?im \<rightarrow> ?f\<close>)
+   (is ?slow is \<open>?c \<in> [?pre]\<^sub>a ?im \<rightarrow> ?f\<close>) and
+  resolve_lookup_conflict_merge_code_set_conflict_fast[sepref_fr_rules]:
+    \<open>(uncurry6 set_lookup_conflict_aa_fast_code, uncurry6 set_conflict_m) \<in>
+  [\<lambda>((((((M, N), i), xs), clvls), lbd), outl). clvls = 0 \<and> i \<in># dom_m N \<and> xs = None \<and> distinct (N \<propto> i) \<and>
+    literals_are_in_\<L>\<^sub>i\<^sub>n (mset (N \<propto> i)) \<and> \<not> tautology (mset (N \<propto> i)) \<and> literals_are_in_\<L>\<^sub>i\<^sub>n_trail M \<and>
+     no_dup M \<and> out_learned M None outl]\<^sub>a
+  trail_fast_assn\<^sup>k *\<^sub>a clauses_ll_assn\<^sup>k *\<^sub>a uint32_nat_assn\<^sup>k *\<^sub>a option_lookup_clause_assn\<^sup>d *\<^sub>a uint32_nat_assn\<^sup>k *\<^sub>a
+      lbd_assn\<^sup>d *\<^sub>a out_learned_assn\<^sup>d \<rightarrow>
+    option_lookup_clause_assn *a uint32_nat_assn *a lbd_assn *a out_learned_assn\<close>
+   (is ?fast is \<open>?cfast \<in> [?pre]\<^sub>a ?imfast \<rightarrow> ?ffast\<close>) 
 proof -
    have H: \<open>?c
   \<in> [comp_PRE (\<langle>Id\<rangle>list_rel \<times>\<^sub>f Id \<times>\<^sub>f nat_rel \<times>\<^sub>f option_lookup_clause_rel \<times>\<^sub>f
@@ -1157,7 +1162,40 @@ proof -
   have f: \<open>?f' = ?f\<close>
     by (auto simp: list_assn_list_mset_rel_eq_list_mset_assn
        option_lookup_clause_assn_def)
-  show ?thesis
+  show ?slow
+    apply (rule hfref_weaken_pre[OF ])
+     defer
+    using H unfolding im f PR_CONST_def apply assumption
+    using pre ..  
+  have H: \<open>?cfast
+  \<in> [comp_PRE (\<langle>Id\<rangle>list_rel \<times>\<^sub>f Id \<times>\<^sub>f nat_rel \<times>\<^sub>f option_lookup_clause_rel \<times>\<^sub>f
+        nat_rel \<times>\<^sub>f Id \<times>\<^sub>f Id)
+     (\<lambda>((((((M, N), i), xs), clvls), lbd), outl). i \<in># dom_m N \<and> xs = None \<and>
+         distinct (N \<propto> i) \<and> literals_are_in_\<L>\<^sub>i\<^sub>n (mset (N \<propto> i)) \<and> \<not> tautology (mset (N \<propto> i)) \<and>
+         clvls = 0 \<and> out_learned M None outl)
+     (\<lambda>_ ((((((M, N), i), _, xs), _), _), _). i \<in># dom_m N \<and> literals_are_in_\<L>\<^sub>i\<^sub>n_trail M \<and>
+         (\<forall>j<length (N \<propto> i). atm_of (N \<propto> i ! j) < length (snd xs)) \<and> no_dup M \<and>
+         literals_are_in_\<L>\<^sub>i\<^sub>n (mset (N \<propto> i)) \<and> length (N \<propto> i) \<le> uint_max)
+     (\<lambda>_. True)]\<^sub>a
+   hrp_comp ((hr_comp trail_pol_fast_assn trail_pol)\<^sup>k *\<^sub>a clauses_ll_assn\<^sup>k *\<^sub>a uint32_nat_assn\<^sup>k *\<^sub>a
+       conflict_option_rel_assn\<^sup>d *\<^sub>a uint32_nat_assn\<^sup>k *\<^sub>a lbd_assn\<^sup>d *\<^sub>a out_learned_assn\<^sup>d)
+     (\<langle>Id\<rangle>list_rel \<times>\<^sub>f Id \<times>\<^sub>f nat_rel \<times>\<^sub>f option_lookup_clause_rel \<times>\<^sub>f
+         nat_rel \<times>\<^sub>f Id \<times>\<^sub>f Id) \<rightarrow>
+    hr_comp (conflict_option_rel_assn *a uint32_nat_assn *a lbd_assn *a out_learned_assn)
+      (option_lookup_clause_rel \<times>\<^sub>f (nat_rel \<times>\<^sub>f (Id \<times>\<^sub>f Id)))\<close> (is \<open>_ \<in> [?pre']\<^sub>a ?im' \<rightarrow> ?f'\<close>)
+     using hfref_compI_PRE_aux[OF set_lookup_conflict_aa_fast_code.refine[unfolded PR_CONST_def]
+        resolve_lookup_conflict_aa_set_conflict[unfolded PR_CONST_def],
+        OF isasat_input_bounded_axioms]
+     unfolding PR_CONST_def
+     .
+  have im: \<open>?im' = ?imfast\<close>
+    unfolding prod_hrp_comp option_lookup_clause_assn_def
+    by (auto simp: prod_hrp_comp hrp_comp_def hr_comp_invalid)
+
+  have f: \<open>?f' = ?ffast\<close>
+    by (auto simp: list_assn_list_mset_rel_eq_list_mset_assn
+       option_lookup_clause_assn_def)
+  show ?fast
     apply (rule hfref_weaken_pre[OF ])
      defer
     using H unfolding im f PR_CONST_def apply assumption
